lean/deps/galois_stdlib/src/galois/data/bool.lean
@@ -1,0 +1,10 @@
+/- Boolean operations. -/
+
+def bimplies : bool → bool → bool
+| tt y := y
+| ff _ := tt
+
+def band_all : list bool → bool
+| [] := tt
+| (tt::r) := band_all r
+| (ff::r) := ff
