lean/deps/galois_stdlib/src/galois/data/option.lean
@@ -1,0 +1,75 @@
+
+namespace option
+
+section
+
+parameter {α : Type _}
+
+/- Is some as a Prop instead of Boolean -/
+inductive is_some_prop : option α → Prop
+| intro (x:α) : is_some_prop (option.some x)
+
+open decidable
+
+instance is_some_prop.decidable : Π(x:option α), decidable (is_some_prop x)
+| none := is_false (by { intro p, cases p, })
+| (some x) := is_true (is_some_prop.intro x)
+
+
+end
+
+@[simp]
+theorem is_some_prop_none {α : Type _} :
+  (@option.is_some_prop α none) ↔ false :=
+begin
+  apply iff.intro,
+  { intro x, cases x, },
+  { intro x, exact (false.elim x), },
+end
+
+@[simp]
+theorem is_some_prop_map {α β : Type _} (x:option α) (f:α → β) :
+  option.is_some_prop (option.map f x) ↔ option.is_some_prop x :=
+begin
+  cases x; simp [option.map, option.bind],
+  case option.some : x {
+    apply iff.intro; intro p; apply (is_some_prop.intro _),
+  },
+end
+
+/- Get the value assuming we have a proof. -/
+def is_some_prop.get {α} : Π{x:option α}, is_some_prop x → α
+| none p :=
+  begin
+    apply false.elim,
+    cases p,
+  end
+| (some x) p := x
+
+@[simp]
+theorem is_some_prop.some_get {α : Type} {x:option α} (p:option.is_some_prop x)
+ : some p.get = x :=
+begin
+  cases p with x,
+  simp [is_some_prop.get],
+end
+
+theorem get_is_some_prop_map {α β : Type _} (x:option α) (f : α → β)
+  (p : option.is_some_prop (option.map f x))
+: f (option.is_some_prop.get ((option.is_some_prop_map x f).mp p))
+  = option.is_some_prop.get p :=
+begin
+  apply option.some.inj,
+  simp [is_some_prop.some_get],
+  cases x,
+  case option.none : {
+    simp at p,
+    exact false.elim p,
+  },
+  case option.some : {
+    simp [is_some_prop.get],
+  },
+end
+
+
+end option
