lean/deps/typed_smt2/src/galois/smt2/test.lean
@@ -7,8 +7,10 @@ open smt2.file_writer
 
 
 def write_test_file : io unit := do
-  smt2.file_writer.run "foo.smt2" $ do
+  smt2.file_writer.run "bar.smt2" $ do
     let x := symbol.of_string "x",
-    declare_const x (bv 32),
-    file_writer.assert (all_equal [bv.decimal (bitvec.of_nat 32 3), var x (bv 32)]),
+    declare_const x (BitVec 32),
+    file_writer.assert (all_equal [bv.decimal (bitvec.of_nat 32 3), var x (BitVec 32)]),
     check_sat
+
+--#eval write_test_file
