lean/deps/typed_smt2/src/galois/smt2/theories/bv.lean
@@ -4,23 +4,14 @@ import ..basic
 
 namespace smt2
 
-/-- SMTLIB bitvec sorts -/
-def bv (w : ℕ) : sort :=
-  { name := symbol.of_string "BitVec"
-  , args := [ident_arg.nat w]
-  , domain := bitvec w
-  , default := 0
-  }
+def term.bv_interp {w:ℕ} (x:term (BitVec w)) (m:interpretation) : bitvec w := x.interp m
 
-def term.bv_interp {w:ℕ} (x:term (bv w)) (m:interpretation) : bitvec w := x.interp m
-
-
-def bv.to_domain {w:ℕ} (d:bitvec w) : (bv w).domain := d
+def bv.to_domain {w:ℕ} (d:bitvec w) : (BitVec w).domain := d
 
 namespace bv
 
 /- Create a term from a decimal number -/
-def decimal {w:ℕ} (v:bitvec w) : term (bv w) :=
+def decimal {w:ℕ} (v:bitvec w) : term (BitVec w) :=
 { to_sexpr := sexpr.parens [ reserved_word.of_string "_"
                            , (symbol.of_string "bv" trivial ++ symbol.of_nat v.to_nat).to_atom
                            , atom.numeral w
@@ -29,13 +20,13 @@ def decimal {w:ℕ} (v:bitvec w) : term (bv w) :=
 }
 
 /-- Bitvector addition -/
-def add {w:ℕ} (x y : term (bv w)) : term (bv w) :=
+def add {w:ℕ} (x y : term (BitVec w)) : term (BitVec w) :=
 { to_sexpr := sexpr.bin_app (symbol.of_string "bvadd" trivial) x y
 , interp := λm, (x.bv_interp m + y.bv_interp m : bitvec w)
 }
 
 /-- Bitvector subtraction -/
-def sub {w:ℕ} (x y : term (bv w)) : term (bv w) :=
+def sub {w:ℕ} (x y : term (BitVec w)) : term (BitVec w) :=
 { to_sexpr := sexpr.bin_app (symbol.of_string "bvsub" trivial) x y
 , interp := λm, (x.bv_interp m - y.bv_interp m : bitvec w)
 }
